EvalLemmas.v
@@ -8,33 +8,47 @@ Require Import SubstLemmas.
 Require Import Types.
 Require Import Judge.
 Require Import Language.
+Require Import ProgramLogic.
 Require Import Tactics.
 
+Open Scope pred.
+
 Lemma var_val : 
-  forall Γ x ν b φ w,  (x,{ ν : b | φ}) ∈ Γ -> 
+  forall Γ x b φ w,  (x,{ ν : b | φ}) ∈ Γ -> 
                        sep_env Γ w -> 
                        (EX v : (base_of_type b), 
                                (fun s => eval s (var_e x) = Some (val_of_base b v))) w.
 Proof.
-  induction Γ; repeat crush_sep False fail.  
+  induction Γ. crush_sep False fail.  
+  crush_sep False fail.
+  fold (subst_pred (subst_one ν (var_e x)) (sep_base ν b0) w) in H.
+  rewrite subst_vv_base_ap in H.
+  apply H.
+  crush_sep False fail.
 Qed.
 
 Lemma var_eval :
-  forall Γ x t w, (x,t) ∈ Γ -> sep_env Γ w -> (EX v : value, (fun s => eval s (var_e x) = Some v)) w.
+  forall Γ x b φ w, (x, { ν : b | φ }) ∈ Γ -> sep_env Γ w -> (EX v : value, (fun s => eval s (var_e x) = Some v)) w.
 Proof.
-  destruct t as [ν b φ]; crush_sep var_val fail.
+  crush_sep False fail.
+  apply var_val with (x := x) (b := b) (φ := φ)in H0 .
+  destruct H0.
+  destruct b. simpl in *. exists (int_v x0). assumption.
+              simpl in *. exists (bool_v x0). assumption.
+  assumption. 
 Qed.
 
 Lemma expr_eval : 
-  forall Γ e T w, 
-    sep_env Γ w -> expr_type Γ e T ->
+  forall Γ e b φ w, 
+    sep_env Γ w -> expr_type Γ e { ν : b | φ } ->
                 (EX v : value, (fun s => eval s e = Some v)) w.
 Proof.
-  autounfold in *. intros. crush_sep False fail. 
-  destruct e as [v | x]. 
-    crush_sep False fail.
-    inversion H0; apply var_eval with (Γ := Γ) (t:= T);
-    crush.
+  autounfold in *. intros. 
+  inversion H0. 
+  subst.
+  simpl. exists v. reflexivity.
+  subst.
+  apply var_eval with (Γ := Γ) (b := b) (φ := φ); crush.
 Qed.
 
 Lemma expr_eval_ty :
@@ -54,16 +68,89 @@ Proof.
     * simpl. exists n. reflexivity.
     * simpl. exists b. reflexivity.
   + inversion H0. subst.
-    * simpl. pose (var_val Γ v ν b φ w H4 H). assumption.
+    * simpl. pose (var_val Γ v b φ w H4 H). assumption.
 Qed.
 
 Lemma expr_eval_derives :
-  forall Γ e t,
-    expr_type Γ e t -> (sep_env Γ) |-- (EX v : value, (fun s => eval s e = Some v)).
+  forall Γ e b φ, 
+    expr_type Γ e { ν : b | φ } -> (sep_env Γ) |-- (EX v : value, (fun s => eval s e = Some v)).
 Proof.
-  intros Γ e t T w Den_Γ.
+  intros Γ e b φ T w Den_Γ.
   destruct e.
   exists v. reflexivity.
-  apply var_eval with (x := v) (t:=t) in Den_Γ .
-  auto. inversion T. apply H1.
+  apply var_eval with (x := v) (b := b) (φ := φ) in Den_Γ .
+  auto. inversion T. apply H2.
+Qed.
+
+Lemma subst_env_eq_expr:
+  forall G b x e w φ, 
+    expr_type G e { ν : b | φ } ->
+    sep_env G w ->
+    (subst_pred (subst_one x e) (sep_env G)) w ->
+    subst_pred (subst_one x e) (sep_env ((x, { ν : b | var_e ν .= e }) :: G)) w.
+Proof.
+  intros G b x e w φ etype senv H.
+  pose (expr_eval_ty G e b φ w senv etype) as H0.
+  rewrite subst_env_cons.
+  split.
+  unfold subst_pred.
+  unfold subst_one.
+  unfold sep_ty.
+  split.
+  unfold sep_base.
+  unfold subst_one. 
+  destruct H0.
+  exists x0.
+  simpl.
+  destruct (eq_dec ν ν).
+  simpl.
+  destruct (eq_dec x x). assumption. contradiction n; reflexivity. contradiction n; reflexivity.
+
+  unfold sep_pred.
+  destruct H0.
+  destruct b.
+  simpl in x0.
+  simpl in H0.
+  exists (int_v x0).
+  exists (int_v x0).
+  constructor. constructor. constructor.
+  simpl. unfold subst_one. simpl.
+  destruct (eq_dec ν ν).
+  simpl.
+  destruct (eq_dec x x).
+  symmetry.
+  assumption.
+  intuition.
+  intuition.
+  unfold subst_one.
+  destruct e. 
+  simpl. symmetry. apply H0.
+  simpl. inversion etype. subst. simpl. 
+  destruct (eq_dec v ν). simpl. 
+  destruct (eq_dec x x). simpl. 
+  symmetry. apply H0.
+  intuition.
+  intuition.
+  destruct (eq_dec v x). symmetry. apply H0. symmetry. apply H0.
+  
+  simpl in *.
+  symmetry in H0.
+  exists (bool_v x0).
+  exists (bool_v x0).
+  repeat constructor.
+  unfold subst_one. 
+  destruct (eq_dec ν ν).
+  simpl.
+  destruct (eq_dec x x).
+  simpl.
+  apply H0. intuition. intuition.
+  destruct e.
+  apply H0.
+  simpl. inversion etype. subst. 
+  unfold subst_one.
+  destruct (eq_dec v ν). simpl.
+  destruct (eq_dec x x). 
+  apply H0. intuition.
+  destruct (eq_dec v x). apply H0. apply H0.
+  assumption.
 Qed.
