Lang.v
@@ -1,0 +1,107 @@
+(**  Module defining the programming languages:
+     - Values
+     - Expressions
+     - Statements **)
+
+Add LoadPath "vst".
+Require Import Arith.
+Require Import List.
+Require Import msl.eq_dec.
+Import Relations. 
+
+Delimit Scope lang_scope with lang.
+
+Definition var := nat.
+
+Inductive value : Set :=
+  | int_v  : nat -> value
+  | bool_v : bool -> value.
+
+(* Inductive bop := *)
+(*   | plus_o : bop. *)
+
+(* (** First we will need a notion of expressions in the language **) *)
+(* Inductive expr :=  *)
+(*   | value_e : value -> expr *)
+(*   | var_e   : var -> expr *)
+(*   | bop_e   : expr -> bop -> expr -> expr. *)
+
+(* Fixpoint subst_expr (x:var) (e':expr) (e:expr) :=  *)
+(*   match e with *)
+(*     | var_e x' =>  *)
+(*       if eq_dec x' x then e' else e *)
+(*     | bop_e e1 o e2 =>  *)
+(*       bop_e (subst_expr x e' e1) o (subst_expr x e' e2) *)
+(*     | _ => e *)
+(*   end. *)
+      
+
+(** Statements: all the fun stuff *)
+Inductive stmt :=
+  | skip_s   : stmt
+  (* | assign_s : var -> expr -> stmt *)
+  | seq_s    : stmt -> stmt -> stmt.
+
+Coercion int_v: nat >-> value.
+Coercion value_e: value >-> expr.
+Coercion var_e: var >-> expr.
+Notation "x .+ y" := (bop_e x plus_o y) (at level 57, right associativity).
+
+(**** Semantics ****)
+(*** a la Appel, PLFCC ***)
+Definition table (A B : Type) := list (A * B).
+Fixpoint table_get {A B}{H: EqDec A} (rho: table A B) (x: A) : option B :=
+  match rho with
+  | (y,v)::ys => if eq_dec x y then Some v else table_get ys x
+  | nil => None
+ end.
+
+Definition table_set {A B}{H: EqDec A} (x: A) (v: B) (rho: table A B)  : table A B := (x,v)::rho.
+
+Lemma table_gss {A B}{H: EqDec A}: forall rho x (v: B), table_get (table_set x v rho) x = Some v.
+Proof.
+intros.
+simpl. destruct (eq_dec x x); auto. contradiction n; auto.
+Qed.
+
+Lemma table_gso {A B}{H: EqDec A}: forall rho x y (v:B), x<>y -> table_get (table_set x v rho) y = table_get rho y.
+Proof.
+intros.
+simpl. destruct (eq_dec y x); auto.  contradiction H0; auto.
+Qed.
+
+Definition state := table var value.
+
+Definition apply_op' o v1 v2 := 
+  match (o, v1, v2) with
+    | (plus_o, int_v v1', int_v v2') => 
+      Some (int_v (v1' + v2'))
+    | _ =>
+      None
+  end.
+
+Definition apply_op o v1 v2 :=
+  match (v1, v2) with
+    | (Some v1', Some v2') => apply_op' o v1' v2'
+    | _ => None
+  end.
+
+Fixpoint eval s e :=
+  match e with
+  | value_e v       => Some v
+  | var_e   x       => s x
+  | bop_e   e1 o e2 => apply_op o (eval s e1) (eval s e2)
+  end.
+
+Inductive step : relation (list stmt * state) :=
+  | step_skip : 
+      forall k s,
+        step (skip_s :: k, s) (k, s)
+  | step_assign :
+      forall k s x e v,
+      Some v = eval (table_get s) e -> 
+      step (assign_s x e :: k, s) (k, table_set x v s)
+  | step_seq :
+      forall k s c1 c2 cs',
+        step (c1 :: c2 :: k, s) cs' ->
+        step (seq_s c1 c2 :: k, s) cs'.
