SubstLemmas.v
@@ -2,227 +2,369 @@ Add LoadPath "vst".
 Require Import msl.msl_direct.
 Require Import Coq.Unicode.Utf8.
 
-Require Import Translation.
 Require Import Types.
 Require Import Judge.
 Require Import Language.
+Require Import ProgramLogic.
+Require Import Translation.
 Require Import Subst.
 Require Import WFLemmas.
 Require Import Tactics.
 
-Lemma subst_none_base :
-  forall x e x' t' s,
-   x <> x' -> (subst_pred x e (sep_base x' t') s) -> (sep_base x' t' s).
+Open Scope pred.
+Lemma subst_empty : 
+  forall p sub,
+    (forall x, sub x = None) ->
+    subst_pred sub p = p.
 Proof.
-  autounfold in *; crush_sep False fail; destruct (eq_dec x x') eqn:EQ; crush.
+  intros. unfold subst_pred. extensionality w. 
+  f_equal. extensionality i. 
+  specialize (H i).
+  rewrite H. reflexivity.
 Qed.
 
-Lemma subst_none_base' :
-  forall x e x' t' s,
-   x <> x' -> (sep_base x' t' s) -> (subst_pred x e (sep_base x' t') s).
-Proof.
-  autounfold in *; crush_sep False fail; destruct (eq_dec x x') eqn:EQ; crush.
-Qed.
+Ltac invProp e1 e2 :=
+        match goal with
+          | [ H : wf_prop _ (rel_r e1 _ e2) |- _ ] =>
+            inversion H;
+            match goal with
+                | [ H : wf_expr _ e1 |- _ ] => inversion H
+                | [ H : wf_expr _ e2 |- _ ] => inversion H
+            end
+        end.
 
-Lemma not_prop_1 :
-  forall φ w,
-    sep_pred (not_r φ) w -> (sep_pred φ) w -> FF w.
-Proof.
-  crush.
-Qed.
+Ltac invTypes :=
+  match goal with
+    | [ H : wf_type _ { _ : _ | (rel_r ?e1 _ ?e2) } |- _ ] => 
+      inversion H; invProp e1 e2
+    | [ H : wf_prop _ (rel_r ?e1 _ ?e2) |- _ ] =>
+      invProp e1 e2
+  end; subst.
 
-Lemma not_prop_2 :
-  forall φ w,
-    sep_pred φ w -> FF w -> sep_pred (not_r φ) w.
-Proof.
-  crush.
-Qed.
+Ltac nonsense_var :=
+  match goal with
+    | [ H : var_not_in ?x _, G: (?v, ?t) ∈ _, X: ?x = ?v |- _ ] =>
+      exfalso;
+      unfold var_not_in in H; 
+      rewrite Forall_forall in H;
+      specialize (H (v,t)); 
+      intuition
+    | [ H : var_not_in ?x _, G: (?v, ?t) ∈ _, X: ?v = ?x |- _ ] =>
+      exfalso;
+      unfold var_not_in in H; 
+      rewrite Forall_forall in H;
+      specialize (H (v,t)); 
+      intuition
+    | [ H : wf_expr _ (var_e ?v), C : var_not_in ?v ?G |- _ ] =>
+      exfalso; 
+      inversion H; 
+      unfold var_not_in in C;
+      rewrite Forall_forall in C; 
+      solve [match goal with
+               | [ _ : (?v, ?t) ∈ ?G |- _ ] => specialize (C (v,t)); intuition
+               | _ => intuition  
+             end]
+    | _ => contradiction; reflexivity
+  end.
+
+Hint Unfold subst_pred.
+Hint Unfold subst_one.
+Hint Unfold exp.
+Hint Unfold andp.
+Hint Unfold orp.
+Hint Unfold imp.
+Hint Unfold prop.
   
-Lemma subst_not :
-  forall x e φ w,
-    subst_pred x e (sep_pred (not_r φ)) w -> (subst_pred x e (sep_pred φ) w -> FF w).
+Ltac break_subst := 
+  simpl; autounfold; 
+  first 
+    [ reflexivity 
+    | subst; nonsense_var
+    | match goal with 
+        | |- appcontext[eq_dec ?x ?y] => 
+          destruct (eq_dec x y); subst; break_subst
+        | |- context[match (?θ ?v) with
+                       | Some _ => _
+                       | None => _
+                     end] =>
+          let Z := fresh "Z" in destruct (θ v) eqn: Z; break_subst
+        | [ Z : ?s ?v = Some _, E : disj_subst ?G ?s, H : wf_expr ?G (var_e ?v)
+          |- _ ] => 
+            unfold disj_subst in E;
+            destruct E as [ E1 E2 ];
+            inversion H;
+            match goal with
+              | _ => subst; rewrite E1 in Z; inversion Z
+              | [ H2 : (?v, ?t) ∈ ?G |- _ ] =>
+                let H3 := fresh "H" in
+                assert (H3: var_in v G) by (exists t; assumption);
+                  specialize (E2 v H3);
+                  rewrite E2 in Z;
+                  inversion Z
+            end
+        | [ H : Some _ = None |- _ ] => inversion H
+        | [ H : None = Some _ |- _ ] => inversion H
+      end].
+
+Lemma subst_singleton :
+  forall G p x e,
+    x <> ν -> var_not_in x G -> wf_prop G p ->
+    (forall w, subst_pred (subst_one x e) (sep_pred p) w = (sep_pred p) w).
 Proof.
-  crush.
+  induction p.
+  + intros; reflexivity.
+  + intros;
+    match goal with 
+      | [ H: wf_prop _ (rel_r ?e ?b ?e0) |- appcontext[rel_r ?e ?b ?e0] ] =>
+        inversion H; destruct e; destruct e0; destruct b; break_subst
+    end.
+  + intros. simpl. unfold imp. inversion H1. specialize (IHp x e H H0 H4). rewrite <- IHp. reflexivity.
+  + intros. simpl. unfold subst_pred. unfold andp. 
+    inversion H1. 
+    specialize (IHp1 x e H H0 H5).
+    specialize (IHp2 x e H H0 H6).
+    fold (subst_pred (subst_one x e) (sep_pred p1) w).
+    fold (subst_pred (subst_one x e) (sep_pred p2) w).
+    rewrite <- IHp1.
+    rewrite <- IHp2.
+    reflexivity.
+  + intros. simpl. unfold imp. inversion H1.
+    specialize (IHp1 x e H H0 H5).
+    specialize (IHp2 x e H H0 H6).
+    simpl. unfold orp. rewrite <- IHp1. rewrite <- IHp2. reflexivity.
 Qed.
 
-Lemma not_inv:
-  forall p q w,
-    sep_pred p w -> sep_pred q w -> sep_pred (not_r q) w -> sep_pred (not_r p) w.
+Lemma subst_empty_dom_base :
+  forall x b θ,
+    θ x = None -> 
+    forall w, 
+      (subst_pred θ (sep_base x b) w = sep_base x b w).
 Proof.
-  crush.
+  intros.
+  unfold sep_base.
+  simpl. autounfold. rewrite H. reflexivity.
 Qed.
 
-Lemma not_inv2:
-  forall p q w,
-    sep_pred p w -> sep_pred (not_r q) w -> sep_pred q w -> sep_pred (not_r p) w.
+Lemma subst_empty_dom_pred :
+  forall G p θ,
+    disj_subst G θ -> 
+    wf_prop G p ->
+    forall w, 
+      (subst_pred θ (sep_pred p) w = sep_pred p w).
 Proof.
-  crush.
+  intros.
+  induction p.
+  + constructor.
+  + inversion H0. destruct e; destruct e0; destruct b; break_subst.
+  + simpl. autounfold. rewrite <- IHp. reflexivity. inversion H0; assumption.
+  + simpl; autounfold; inversion H0. rewrite <- IHp1. rewrite <- IHp2. reflexivity. 
+    assumption. assumption.
+  + simpl; autounfold; inversion H0. rewrite <- IHp1. rewrite <- IHp2. reflexivity.
+    assumption. assumption.
 Qed.
 
-Lemma subst_none_eq :
-  forall x e Γ ν τ e1 e2 s,
-    var_not_in x Γ -> wf_type Γ { ν : τ | e1 .= e2 } -> (x <> ν) -> 
-    (subst_pred x e (sep_pred (e1 .= e2)) s <-> sep_pred (e1 .= e2) s).
-    (* /\ (sep_pred (e1 .= e2) s -> subst_pred x e (sep_pred (e1 .= e2)) s)). *)
+  
+Lemma subst_vv_pred :
+  forall G p x θ,
+    disj_subst G θ -> wf_prop G p -> 
+    forall w,
+    (subst_pred (subst_one ν (var_e x)) (subst_pred θ (sep_pred p)) w
+               =
+    subst_pred (subst_one ν (var_e x)) (sep_pred p) w).
 Proof.
-  unfold subst_pred;
-  crush' var_not_in_exp (wf_expr, wf_prop, wf_type);
-  destruct e1 eqn:E1; 
-  destruct e2 eqn:E2;
-  crush_sep False fail;
-    repeat match goal with
-             | [ H: context[eq_dec ?x ?y] |- _ ] => destruct (eq_dec x y)
-             | |- context[eq_dec ?x ?y] => destruct (eq_dec x y)
-             | |- appcontext[( _ && _ )] => split; simpl
-          end; crush.
-Qed.
-
-Lemma subst_none_lt :
- forall x e Γ ν τ e1 e2 s,
-    var_not_in x Γ -> wf_type Γ { ν : τ | e1 .< e2 } -> x <> ν ->
-    (subst_pred x e (sep_pred (e1 .< e2)) s <-> sep_pred (e1 .< e2) s).
-Proof.
-  unfold subst_pred;
-  crush' var_not_in_exp (wf_expr, wf_prop, wf_type);
-  destruct e1;
-  destruct e2;
-  reduce_preds;
-    repeat (match goal with
-              | [ x:_, y:_, H:appcontext[!!(?x < ?y)] |- _] => exists x; exists y; simpl
-              | [ H: context[eq_dec ?x ?y] |- _ ] => destruct (eq_dec x y)
-              | |- context[eq_dec ?x ?y] => destruct (eq_dec x y)
-              | |- appcontext[( _ && _ )] => split; simpl
-            end; crush).
-Qed.
-
-Lemma subst_none_rel :
- forall x e Γ ν τ b e1 e2 s,
-    var_not_in x Γ -> wf_type Γ { ν : τ | rel_r e1 b e2 } -> x <> ν ->
-    (subst_pred x e (sep_pred (rel_r e1 b e2)) s <-> sep_pred (rel_r e1 b e2) s).
-Proof.
-  destruct b. apply subst_none_eq. apply subst_none_lt.
-Qed.
-
-Lemma subst_not_1 :
-  forall φ s,
-    (sep_pred (not_r φ) s -> (sep_pred φ s -> FF s)).
-Proof.
-  crush.
-Qed.
-
-Lemma subst_not_2 :
-  forall φ s,
-    (sep_pred φ s -> FF s) -> (sep_pred (not_r φ) s).
-Proof.
-  crush.
-Qed.
-
-Lemma subst_none_prop :
-  forall φ x e Γ τ s,
-    var_not_in x Γ -> wf_type Γ { ν : τ | φ } -> x <> ν ->
-    (subst_pred x e (sep_pred φ) s <-> sep_pred φ s).
-Proof.
-  Ltac autocons := 
-    repeat (econstructor || app_pred || eauto); crush.
-  Ltac t :=
-    first [btapply autocons | solve [left; btapply autocons] | solve [right; btapply autocons]].
-  intro φ.
-  induction φ.
-  (* true *)
-  crush. 
-  (* rel *)
-  intros; apply subst_none_rel with (Γ := Γ) (ν := ν) (τ := τ); auto.
-  (* not *)
-  wf_crush; t.
-  (* and  *)
-  wf_crush; t.
-  (* or *)
-  wf_crush; t. 
-Qed.
-
-Lemma subst_commute :
-  forall (x y : var) (x' y' : expr) p s,
-    (var_e y) <> x' -> (var_e x) <> y' -> x <> y -> x' <> y' ->
-    subst_pred x x' (subst_pred y y' p) s =
-      subst_pred y y' (subst_pred x x' p) s.
-Proof.
-  intros. unfold subst_pred. f_equal.
-  destruct x' as [x'v | x']. 
-    extensionality. simpl.
-      destruct y' as [y'v | y'].
-        destruct (eq_dec x x0). 
-          destruct (eq_dec y x0). 
-            rewrite e in H1. rewrite e0 in H1. exfalso. apply H1; reflexivity.
-            reflexivity.
-          destruct (eq_dec y x0).
-            rewrite e in H1. reflexivity.
-            reflexivity.
-        destruct (eq_dec x x0).
-          destruct (eq_dec y x0). 
-            rewrite e in H1. rewrite e0 in H1. exfalso. apply H1; reflexivity.
-            reflexivity.
-          destruct (eq_dec y x0). 
-            simpl. destruct (eq_dec x y'). 
-              rewrite e0 in H0. contradiction H0. reflexivity.
-              reflexivity.
-            reflexivity.
-    extensionality. simpl.
-      destruct y' as [y'v | y'].
-        destruct (eq_dec y x0).
-          simpl. destruct (eq_dec x x0).
-            rewrite e in H1. rewrite e0 in H1. contradiction H1. reflexivity.
-            reflexivity. 
-        destruct (eq_dec x x0). simpl.
-          destruct (eq_dec y x'). 
-            rewrite e0 in H. contradiction H. reflexivity.
-            reflexivity.
-          reflexivity.
-       destruct (eq_dec y x0). simpl.
-         destruct (eq_dec x y'). rewrite e0 in H0. contradiction H0. reflexivity.
-         destruct (eq_dec y x'). rewrite e0 in H. contradiction H. reflexivity. 
-         destruct (eq_dec x x0). rewrite e in H1. rewrite e0 in H1. contradiction H1. reflexivity.
-         reflexivity.
-         destruct (eq_dec y x'). rewrite e in H. contradiction H. reflexivity.
-         reflexivity.
-Qed.
-
-Lemma subst_none_ty : 
-  forall Γ x x' e T s, 
-    x <> ν -> x' <> ν -> var_e ν <> e -> x <> x' ->
-    var_not_in x Γ -> wf_type Γ T -> var_in x' Γ ->
-    (subst_pred x e (sep_ty x' T) s -> sep_ty x' T s).
-Proof.
-  intros Γ x x' e T s neq_x_vv neq_x'_vv neq_e_vv neq_x_x' NotIn WF_Type VarIn.
-  inversion WF_Type; subst.
-  intro SubSep; destruct SubSep as [SepBase SepTy]; apply subst_none_base in SepBase.
-  unfold sep_ty. split. assumption.
-  fold (subst_pred x e (sep_pred (subst ((ν,x')::nil) p)) s) in SepTy.
-  pose subst_none_prop as Foo.
-  specialize (Foo (subst ((ν,x') :: nil) p) x e Γ b s NotIn).
-  apply Foo.
-  apply wf_reft_t. apply wf_prop_subst. 
-  assumption.
-  assumption.
-  assumption.
+  intros.
+  apply subst_empty_dom_pred with (G := G).
   assumption.
   assumption.
 Qed.
 
-Lemma subst_none_ty' :
-  forall Γ x x' e T s, 
-    x <> ν -> x' <> ν -> var_e ν <> e -> x <> x' ->
-    var_not_in x Γ -> wf_type Γ T -> var_in x' Γ ->
-    (sep_ty x' T s -> subst_pred x e (sep_ty x' T) s ).
+Lemma subst_vv_pred' :
+  forall G p x θ,
+    disj_subst G θ -> wf_prop G p -> θ x = None -> 
+    forall w,
+    (subst_pred θ (subst_pred (subst_one ν (var_e x)) (sep_pred p)) w
+               =
+    subst_pred (subst_one ν (var_e x)) (sep_pred p) w).
 Proof.
-  intros Γ x x' e T s neq_x_vv neq_x'_vv neq_e_vv neq_x_x' NotIn WF_Type VarIn.
-  inversion WF_Type; subst.
-  intro SepTy. destruct SepTy as [SepBase SepPred].
-  apply subst_none_base' with (x := x) (e := e) (x' := x') (t' := b) in SepBase.
-  2: assumption.
-  unfold sep_ty.
-  split. assumption.
-  pose subst_none_prop as foo.
-  specialize (foo (subst ((ν,x')::nil) p) x e Γ b s NotIn). 
-  apply foo.
-  apply wf_reft_t. apply wf_prop_subst. assumption. assumption. assumption. assumption.
+  intros.
+  induction p.
+  + constructor.
+  + inversion H0.
+    destruct e; destruct e0; destruct b; break_subst.
+  + intros. simpl.
+    unfold FF.
+    unfold prop.
+    unfold imp.
+    unfold subst_pred at 3. 
+    fold (subst_pred (subst_one ν (var_e x)) (sep_pred p) w).
+    rewrite <- IHp.
+    reflexivity.
+    inversion H0.
+    assumption.
+  + intros. inversion H0.
+    specialize (IHp1 H5). specialize (IHp2 H6).
+    simpl.
+    unfold andp.
+    unfold subst_pred at 3.
+    fold (subst_pred (subst_one ν (var_e x)) (sep_pred p1) w).
+    fold (subst_pred (subst_one ν (var_e x)) (sep_pred p2) w).
+    rewrite <- IHp1.
+    rewrite <- IHp2.
+    reflexivity.
+  + intros. inversion H0.
+    specialize (IHp1 H5).
+    specialize (IHp2 H6).
+    simpl.
+    unfold orp.
+    unfold subst_pred at 3.
+    fold (subst_pred (subst_one ν (var_e x)) (sep_pred p1) w).
+    fold (subst_pred (subst_one ν (var_e x)) (sep_pred p2) w).
+    rewrite <- IHp1.
+    rewrite <- IHp2.
+    reflexivity.
+Qed.
+
+Lemma subst_vv_base :
+  forall b x w θ,
+    θ ν = None ->
+    subst_pred (subst_one ν (var_e x)) (subst_pred θ (sep_base ν b)) w
+               =
+    subst_pred (subst_one ν (var_e x)) (sep_base ν b) w.
+Proof.
+  intros.
+  unfold sep_base.
+  autounfold.
+  simpl. rewrite H. destruct (eq_dec ν ν). reflexivity. contradiction n. reflexivity.
+Qed.
+
+Lemma subst_vv_base' :
+  forall b x w θ,
+    θ ν = None -> θ x = None ->
+    subst_pred θ (subst_pred (subst_one ν (var_e x)) (sep_base ν b)) w
+               =
+    subst_pred (subst_one ν (var_e x)) (sep_base ν b) w.
+Proof.
+  intros.
+  unfold sep_base.
+  autounfold.
+  simpl.
+  destruct (eq_dec ν ν). simpl. rewrite H0. reflexivity.
+  rewrite H. reflexivity.
+Qed.
+
+Lemma subst_vv_base_ap :
+  forall b x w,
+    subst_pred (subst_one ν (var_e x)) (sep_base ν b) w
+    = sep_base x b w.
+Proof.
+  intros.
+  unfold sep_base.
+  unfold subst_pred.
+  unfold exp. 
+  unfold subst_one.
+  simpl.
+  destruct (eq_dec ν ν).
+  simpl. reflexivity.
+  contradiction n.
+  reflexivity.
+Qed.
+
+Lemma sep_ty_split :
+  forall x b p,
+    forall w, (sep_ty x { ν : b | p } w =
+    ((subst_pred (subst_one ν (var_e x)) (sep_base ν b)) w 
+    /\ (subst_pred (subst_one ν (var_e x)) (sep_pred p) w))).
+Proof.
+  intros.
+  split.
+Qed.
+
+Lemma subst_ty :
+  forall G b p x θ w,
+    disj_subst G θ -> wf_type G { ν : b | p } -> θ x = None -> θ ν = None ->
+      (subst_pred θ (sep_ty x { ν : b | p }) w
+       =
+       sep_ty x { ν : b | p } w).
+Proof.
+  intros.
+  unfold subst_pred.
+  rewrite sep_ty_split.
+  rewrite sep_ty_split.
+  fold (subst_pred θ (subst_pred (subst_one ν (var_e x)) (sep_pred p)) w).
+  fold (subst_pred θ (subst_pred (subst_one ν (var_e x)) (sep_base ν b)) w).
+  f_equal. 
+  rewrite <- subst_vv_base' with (θ := θ). 
+    reflexivity. assumption. assumption.
+  rewrite <- subst_vv_pred' with (G := G) (θ := θ). 
+    reflexivity. assumption. apply wf_type_prop with (ν := ν) (τ := b).
+    assumption. assumption.
+Qed.
+
+Lemma disj_subst_cons :
+  forall G x t θ,
+    disj_subst ((x,t) :: G) θ -> disj_subst G θ.
+Proof.
+  induction G.
+  + intros. 
+    unfold disj_subst in *.
+    destruct H.
+    split.
+    assumption.
+    intros.
+    unfold var_in in H1.
+    destruct H1.
+    inversion H1.
+  + intros.
+    unfold disj_subst in *.
+    destruct H.
+    split.
+    assumption.
+    destruct a.
+    intros.
+    apply H0.
+    unfold var_in in H1.
+    unfold var_in.
+    destruct H1.
+    unfold In.
+    unfold In in H1.
+    destruct H1. inversion H1. subst.
+    exists x1. right. left. assumption.
+    fold (In (x0, x1) G) in H1.
+    exists x1.
+    right.
+    right.
+    assumption.
+Qed.
+
+Lemma subst_dom_env :
+  forall G θ,
+    wf_env G -> disj_subst G θ -> θ ν = None -> 
+    forall w,
+      subst_pred θ (sep_env G) w = sep_env G w.
+Proof.
+  induction G.
+  + intros. reflexivity.
+  + intros. destruct a. unfold sep_env. unfold andp.
+    unfold subst_pred. f_equal. 
+    fold (subst_pred θ (sep_ty v r) w).
+    inversion H. inversion H8. subst.
+    apply subst_ty with (G := G).
+    unfold disj_subst in H0.
+    apply disj_subst_cons with (x := v) (t := { ν : b | p } ).
+    assumption.
+    assumption.
+    apply H0. unfold var_in. exists { ν : b | p }. left. reflexivity.
+    assumption.
+    apply IHG. 
+    inversion H. assumption.
+    apply disj_subst_cons in H0. apply H0.
+    assumption.
+Qed.
+
+Lemma subst_env_cons : 
+  forall G θ x t w,
+      (subst_pred θ (sep_env ((x,t) :: G)) w) = 
+                    (subst_pred θ (sep_ty x t) w /\ subst_pred θ (sep_env G) w).  
+Proof.
+  reflexivity.
 Qed.
